coq/ExtractProofState.v
@@ -15,7 +15,7 @@ Set Extraction Output Directory "extracted".
 Extraction "proof_state.ml"
   start state_goals
   step run rule_step rule_run
-  named_start named_goals named_solved
+  named_start_with_constants named_start named_goals named_solved
   named_step named_run named_rule_step named_rule_run
   named_default_all_intro_rule_step
   named_fixed_axiom_rule_step
@@ -24,9 +24,10 @@ Extraction "proof_state.ml"
   named_separation_tactic_step
   named_replacement_tactic_step
   named_execute_rule
-  certified_start certified_goals certified_solved
+  certified_start_with_constants certified_start certified_goals certified_solved
   one_step certified_step certified_run
-  certified_certificate replay_certificate certified_finalize
+  certified_certificate
+  replay_certificate_with_constants replay_certificate certified_finalize
   certified_execute_rule
   certified_separation_tactic
   certified_replacement_tactic
